various work

theories/case_studies/generator_iterator.v
@@ -17,10 +17,10 @@ From affect.lang Require Import affect.
 From affect.logic Require Import sem_def.
 From affect.logic Require Import sem_env.
 From affect.logic Require Import sem_sig.
+From affect.logic Require Import mode.
 From affect.logic Require Import sem_row.
 From affect.logic Require Import sem_judgement.
 From affect.logic Require Import sem_types.
-From affect.logic Require Import copyable.
 From affect.logic Require Import sem_operators.
 From affect.logic Require Import tactics.
 From affect.logic Require Import compatibility.
@@ -58,13 +58,27 @@ Definition iterate :=
         |  SOME "x" => "f" "x" ;; "go" "g" 
         end) "g"))%V.
 
+Definition list_iter :=
+    (Λ: Λ: λ: "xs",
+      (Λ: (λ: "f", 
+            (rec: "go" "xs" := 
+              list-match: "xs" with
+                CONS "x" => "xxs" => ("f" "x" ;; "go" "xxs")
+              | NIL => #()
+              end) "xs"
+         ))
+    )%V.
+
 Section typing.
 
   Context `{!heapGS Σ}.
 
   Definition yield_sig (τ : sem_ty Σ) : operation * sem_sig Σ := ("yield", ∀S: (_ : sem_ty Σ), τ =[OS]=> ())%S.
-  Definition yield_ty τ := τ -{ (yield_sig τ · ⟨⟩) }-> ().
-  Definition iter_ty τ := (∀M: m, ∀R: θ, ('!_[m] τ -{ ¡_[m] θ }-> ()) -{ ¡_[m] θ }-[m]-> ())%T.
+  Definition yield_ty τ := τ -{ ¡ (yield_sig τ · ⟨⟩) }-> ().
+  Definition iter_ty τ := (∀R:[OS] θ, (τ -{ ¡ θ }-> ()) -{ ¡ θ }-∘ ())%T.
+  Definition iter_ty_un τ := (∀R: θ, (τ -{ θ }-> ()) -{ θ }-> ())%T.
+  Definition iter_ty_gen m τ := (∀R:[m] θ, ('!_[m] τ -{ ¡_[m] θ }-> ()) -{ ¡_[m] θ }-[m]-> ())%T.
+  Definition list_iter_ty := (∀M: ν, ∀T: α, List ('!_[ν] α) → iter_ty_gen ν α).
   Definition generator_ty τ := (() → Option τ)%T.
   
   Lemma sem_typed_generate :
@@ -72,18 +86,19 @@ Section typing.
   Proof.
     iIntros "". iApply sem_typed_Tclosure. iIntros (α).
     rewrite -(app_nil_r []). iApply sem_typed_ufun; solve_sidecond. simpl.
-    set cont_ty := (() -{ yield_sig α · ⟨⟩ }-∘ ()). 
+    set cont_ty := (() -{ ¡ (yield_sig α · ⟨⟩) }-∘ ()). 
     iApply (sem_typed_let (Refᶜ cont_ty) _ _ _ []); simpl; solve_sidecond. 
     - iApply sem_typed_alloc_cpy.
       rewrite -(app_nil_r [("i", _)]).
       iApply sem_typed_afun; solve_sidecond. 
       iApply (sem_typed_app_os (yield_ty α) _ _ _ [("i", iter_ty α)]); solve_sidecond.
       + iApply sem_typed_sub_nil.
-        iApply (sem_typed_RApp (λ ρ, ( α -{ ρ }-> ()) -{ ρ }-∘ ())); solve_sidecond.
+        iApply (sem_typed_RApp (λ ρ, ( α -{ ¡ ρ }-> ()) -{ ¡ ρ }-∘ ())); solve_sidecond.
         iApply sem_typed_var.
       + iApply sem_typed_frame. iApply sem_typed_sub_nil.
         iApply sem_typed_val. rewrite /yield /yield_ty. iApply sem_typed_closure; solve_sidecond.
-        simpl. iApply (sem_typed_perform_os (TT:=[tele _]) [tele_arg ()] with "[]"). 
+        simpl. iApply sem_typed_sub_row; first iApply (row_le_mfbang_intro OS).
+        iApply (sem_typed_perform_os (TT:=[tele _]) [tele_arg ()] with "[]"). 
         iApply sem_typed_var'.
     - set Γ₁ :=[("cont", Refᶜ cont_ty)]; rewrite -(app_nil_r Γ₁). 
       iApply sem_typed_ufun; solve_sidecond. simpl.
@@ -92,13 +107,18 @@ Section typing.
       iApply (sem_typed_shandler (TT:=[tele _]) OS "yield" (tele_app (λ _, α)) (tele_app (λ _, ())) () (Option α) ⊥ _ [("cont", Refᶜ cont_ty)] [] [] [("cont", Refᶜ cont_ty)]); solve_sidecond.
       * iLeft. iPureIntro. apply _.
       * iApply row_le_refl. 
-      * iApply sem_typed_app_os; [|iApply sem_typed_unit']. 
+      * iApply sem_typed_sub_row; first iApply (row_le_mfbang_elim OS).
+        iApply sem_typed_app_os; [|iApply sem_typed_unit']. 
         iApply sem_typed_replace_cpy_os; first iApply sem_typed_var'.
+        iApply sem_typed_sub_nil.
         iApply sem_typed_frame. rewrite -(app_nil_r []).
         iApply sem_typed_sub_nil.
         iApply sem_typed_afun; solve_sidecond.
         simpl. iApply sem_typed_unit'.
       * iIntros (?). do 2 iApply sem_typed_swap_third.
+        rewrite -/(yield_sig α) /cont_ty.
+        iApply sem_typed_sub_env; first iApply env_le_cons; first iApply env_le_refl.
+        { iApply ty_le_aarr; first iApply (row_le_mfbang_intro OS); iApply ty_le_refl. }
         iApply sem_typed_seq.
         { iApply sem_typed_replace_cpy_os; iApply sem_typed_var. }
         iApply sem_typed_some. iApply sem_typed_var.
@@ -127,13 +147,15 @@ Section typing.
         iApply (sem_typed_handler (TT:=[tele _]) OS "yield" (tele_app (λ _, α)) (tele_app (λ _, ())) () (Option α) ⊥ _ [("i", iter_ty α)] [] [] [("cont", Refᶜ cont_ty)]); solve_sidecond.
         * iApply row_le_refl. 
         * iApply (sem_typed_app_os (yield_ty α) _ _ _ [("i", iter_ty α)]); solve_sidecond.
-          ** iApply sem_typed_sub_nil.
-             iApply (sem_typed_RApp (λ ρ, ( α -{ ρ }-> ()) -{ ρ }-∘ ())); solve_sidecond.
+          ** iApply sem_typed_sub_nil. iApply sem_typed_sub_ty.
+             { iApply ty_le_aarr; first iApply (row_le_mfbang_elim OS); iApply ty_le_refl. }
+             iApply (sem_typed_RApp (λ ρ, ( α -{ ¡ ρ }-> ()) -{ ¡ ρ }-∘ ())); solve_sidecond.
              iApply sem_typed_var.
           ** iApply sem_typed_sub_nil.
              iApply sem_typed_frame.
              iApply sem_typed_val. rewrite /yield /yield_ty. iApply sem_typed_closure; solve_sidecond.
-             simpl. iApply (sem_typed_perform_os (TT:=[tele _]) [tele_arg ()] with "[]"). 
+             simpl. iApply sem_typed_sub_row; first iApply (row_le_mfbang_intro OS).
+             iApply (sem_typed_perform_os (TT:=[tele _]) [tele_arg ()] with "[]"). 
              iApply sem_typed_var'.
         * iIntros (?). do 2 iApply sem_typed_swap_third.
           iApply sem_typed_seq.
@@ -156,7 +178,9 @@ Section typing.
   Proof.
     iIntros. iApply sem_typed_closure; first done. rewrite /iter_ty /=.
     rewrite - {1}(app_nil_r [("g", _)]). 
-    iApply sem_typed_RLam; solve_sidecond. iIntros (θ).
+    iApply sem_typed_RLam; simpl; solve_sidecond. 
+    { iApply mode_env_sub_ms; solve_copy. }
+    iIntros (θ).
     rewrite - {1}(app_nil_r [("g", _)]). 
     iApply sem_typed_sub_nil. 
     iApply sem_typed_ufun; solve_sidecond. simpl.
@@ -179,6 +203,58 @@ Section typing.
         iApply sem_typed_var'.
       + iApply sem_typed_app_nil; [|iApply sem_typed_var'].
         iApply sem_typed_sub_u2aarr. iApply sem_typed_var'.
+  Qed.
+
+  Lemma sem_typed_list_iter :
+    ⊢ ⊨ᵥ list_iter : list_iter_ty.
+  Proof.
+    iIntros. rewrite /list_iter /list_iter_ty.
+    iApply sem_typed_Mclosure. iIntros (ν).
+    rewrite - {1}(app_nil_r []).
+    iApply sem_typed_TLam; solve_copy. iIntros (α).
+    rewrite - {1}(app_nil_r []).
+    iApply sem_typed_ufun; solve_sidecond. simpl.
+    rewrite - {1}(app_nil_r [("xs", _)]). 
+    iApply sem_typed_sub_env; first iApply env_le_cons; first iApply env_le_refl.
+    iApply ty_le_list_bang.
+    rewrite - {1}(app_nil_r [("xs", _)]). 
+    iApply sem_typed_RLam. 
+    { iApply mode_env_sub_cons; first iApply mode_env_sub_ms; solve_copy. iApply mode_type_sub_mbang. }
+    iIntros (θ).
+    rewrite - {1}(app_nil_r [("xs", _)]). 
+    iApply sem_typed_fun; solve_sidecond. simpl.
+    { iApply mode_env_sub_cons; first iApply mode_env_sub_ms; solve_copy. iApply mode_type_sub_mbang. }
+    iApply sem_typed_swap_second.
+    iApply sem_typed_sub_env; first iApply env_le_cons; first iApply env_le_refl.
+    { iApply ty_le_mbang_elim. }
+    simpl. rewrite app_singletons.
+    iApply (sem_typed_app_gen (List ('!_[ν] α)) ⟨⟩%R (¡_[ ν ] θ)%R (¡_[ ν ] θ)%R); last iApply sem_typed_var'.
+    - iApply row_le_nil.
+    - iApply row_type_sub_once.
+    - iApply row_env_sub_copy; solve_copy.
+    - iApply row_le_refl.
+    - rewrite - {1}(app_nil_r [("f", _)]). 
+      iApply sem_typed_sub_ty; first iApply ty_le_u2aarr.
+      iApply sem_typed_ufun; solve_sidecond. simpl.
+      iApply (sem_typed_match_list ('!_[ν] α) (¡_[ν] θ)%R _ _ [("go", _); ("f", _)]); solve_sidecond.
+      + iApply sem_typed_var'.
+      + do 2 (iApply sem_typed_weaken). iApply sem_typed_unit'.
+      + iApply (sem_typed_seq () _ _ _ [("go", _); ("xxs", _)]); 
+          last (iApply sem_typed_swap_second; iApply sem_typed_app_nil; [iApply sem_typed_sub_ty; first iApply ty_le_u2aarr|]; iApply sem_typed_var').
+        iApply sem_typed_swap_third. iApply sem_typed_swap_second.
+        iApply sem_typed_swap_fourth. 
+        iApply (sem_typed_app_gen ('!_[ν] α) ⟨⟩%R _ (¡_[ν] θ)%R). 
+        * iApply row_le_nil.
+        * iApply row_type_sub_once.
+        * iApply row_env_sub_cons; last iApply row_type_sub_copy; solve_copy.
+          iApply row_env_sub_cons; last iApply row_type_sub_mfbang_mbang. iApply row_env_sub_copy; solve_copy. 
+        * iApply row_le_refl.
+        * iApply sem_typed_var'.
+        * iApply sem_typed_swap_second. 
+          iApply sem_typed_sub_env_final; last iApply sem_typed_var'. 
+          iApply env_le_cons; last iApply ty_le_u2aarr.
+          iApply env_le_cons; first iApply env_le_cons; first iApply env_le_refl; first iApply ty_le_list_bang.
+          iApply ty_le_uarr; [iApply row_le_refl|iApply ty_le_mbang_elim|iApply ty_le_refl].
   Qed.
 
 End typing.
