theories/logic/mode.v
@@ -13,27 +13,50 @@ From affect.lib Require Import logic.
 From affect.lang Require Import affect.
 From affect.logic Require Import sem_def.
 
-Definition mode_mult m m' : mode :=
+Definition mode_glb m m' : mode :=
+  match m with
+    OS => OS 
+  | MS => m'
+  end.
+
+Definition mode_lub m m' : mode :=
   match m with
     MS => MS
   | OS => m'
   end.
 
-Lemma mode_mult_idemp m :
-  mode_mult m m = m.
+Lemma mode_glb_idemp m :
+  mode_glb m m = m.
 Proof. by destruct m. Qed.
 
-Lemma mode_mult_assoc m₁ m₂ m₃ :
-  mode_mult m₁ (mode_mult m₂ m₃) = (mode_mult (mode_mult m₁ m₂) m₃).
+Lemma mode_glb_assoc m₁ m₂ m₃ :
+  mode_glb m₁ (mode_glb m₂ m₃) = (mode_glb (mode_glb m₁ m₂) m₃).
 Proof. by destruct m₁. Qed.
 
-Lemma mode_mult_comm m₁ m₂ :
-  mode_mult m₁ m₂ = mode_mult m₂ m₁.
+Lemma mode_glb_comm m₁ m₂ :
+  mode_glb m₁ m₂ = mode_glb m₂ m₁.
 Proof. by destruct m₁, m₂. Qed.
 
-Lemma mode_mult_ms m :
-  mode_mult MS m = MS.
+Lemma mode_glb_os m :
+  mode_glb OS m = OS.
 Proof. destruct m; eauto. Qed.
+
+Lemma mode_lub_idemp m :
+  mode_lub m m = m.
+Proof. by destruct m. Qed.
+
+Lemma mode_lub_assoc m₁ m₂ m₃ :
+  mode_lub m₁ (mode_lub m₂ m₃) = (mode_lub (mode_lub m₁ m₂) m₃).
+Proof. by destruct m₁. Qed.
+
+Lemma mode_lub_comm m₁ m₂ :
+  mode_lub m₁ m₂ = mode_lub m₂ m₁.
+Proof. by destruct m₁, m₂. Qed.
+
+Lemma mode_lub_ms m :
+  mode_lub MS m = MS.
+Proof. destruct m; eauto. Qed.
+
 
 (* Sub-Typing on Mode *)
 
@@ -47,21 +70,71 @@ Lemma mode_le_trans {Σ} (m1 m2 m3 : mode) :
 Proof. iIntros "#H12 H23". destruct m1,m2,m3; eauto. Qed.
 
 Lemma mode_le_MS {Σ} (m : mode) : 
-  ⊢ (MS ≤M m : iProp Σ).
+  ⊢ (m ≤M MS : iProp Σ).
 Proof. by iRight. Qed.
 
-Lemma mode_mult_le {Σ} (m₁ m₁' m₂ m₂' : mode) :
+Lemma mode_lub_le {Σ} (m₁ m₁' m₂ m₂' : mode) :
   m₁ ≤M m₁' -∗ m₂ ≤M m₂' -∗
-  mode_mult m₁ m₂ ≤M@{ Σ } mode_mult m₁' m₂'.
+  mode_lub m₁ m₂ ≤M@{ Σ } mode_lub m₁' m₂'.
 Proof. iIntros "Hm₁₁' Hm₂₂'". destruct m₁,m₂,m₁',m₂'; eauto. Qed.
 
 Lemma mode_le_OS {Σ} (m : mode) : 
-  ⊢ (m ≤M OS : iProp Σ).
+  ⊢ (OS ≤M m : iProp Σ).
 Proof. destruct m; eauto. Qed.
 
 Lemma mode_le_OS_inv {Σ} (m : mode) : 
-  (OS ≤M m : iProp Σ) -∗ m ≡ OS.
+  (m ≤M OS : iProp Σ) -∗ m ≡ OS.
 Proof.
   iIntros "H". destruct m; first done.
   iDestruct "H" as "%H". inv H.
+Qed.
+
+Notation "m ⊓ₘ m'" := (mode_glb m m') (at level 80) : bi_scope.
+Notation "m ⊔ₘ m'" := (mode_lub m m') (at level 80) : bi_scope.
+
+Definition mode_type_sub {Σ} (m : mode) (τ : sem_ty Σ) : iProp Σ :=
+  □ (∀ v, τ v -∗ □? m (τ v)).
+
+Notation "m ₘ≼ₜ τ" := (mode_type_sub m τ%T) (at level 80) : bi_scope.
+
+Lemma mode_type_sub_os {Σ} (τ : sem_ty Σ) : ⊢ OS ₘ≼ₜ τ.
+Proof. rewrite /mode_type_sub /=. iIntros "!# % $ //". Qed.
+
+Lemma mode_type_sub_ms {Σ} m (τ : sem_ty Σ) : copy_ty τ ⊢ m ₘ≼ₜ τ.
+Proof. 
+  rewrite /mode_type_sub /=. iIntros "#Hcpy !# % Hτ". 
+  iApply bi.intuitionistically_intuitionistically_if.
+  iApply ("Hcpy" with "Hτ"). 
+Qed.
+
+Definition mode_env_sub {Σ} (m : mode) (Γ : env Σ) : iProp Σ :=
+  □ (∀ γ, ⟦ Γ ⟧ γ -∗ □? m (⟦ Γ ⟧ γ)).
+
+Notation "m ₘ≼ₑ Γ" := (mode_env_sub m Γ%T) (at level 80) : bi_scope.
+
+Lemma mode_env_sub_os {Σ} (Γ : env Σ) : ⊢ OS ₘ≼ₑ Γ.
+Proof. rewrite /mode_env_sub /=. iIntros "!# % $ //". Qed.
+
+Lemma mode_env_sub_ms {Σ} m (Γ : env Σ) : copy_env Γ -∗ m ₘ≼ₑ Γ.
+Proof. 
+  rewrite /mode_env_sub /=. iIntros "#Hcpy !# % HΓ ". 
+  iApply bi.intuitionistically_intuitionistically_if.
+  iApply ("Hcpy" with "HΓ"). 
+Qed.
+
+Lemma mode_env_sub_nil {Σ} m : ⊢ m ₘ≼ₑ ([] : env Σ).
+Proof. iApply mode_env_sub_ms. iIntros "!# % _ //". Qed.
+
+Lemma mode_env_sub_cons {Σ} m x τ (Γ : env Σ) : 
+  m ₘ≼ₑ Γ -∗ m ₘ≼ₜ τ -∗ m ₘ≼ₑ ((x, τ) :: Γ).
+Proof.
+  iIntros "#HmΓ #Hmτ %γ !# (%w & %Heq & Hτ & HΓ)".
+  iSpecialize ("HmΓ" $! γ with "HΓ").
+  iSpecialize ("Hmτ" $! w with "Hτ").
+  Search "intuitionistically_if".
+  iDestruct (bi.intuitionistically_if_sep_2 m (⟦ Γ ⟧ γ) (τ w) with "[HmΓ Hmτ]") as "HmΓτ".
+  { iFrame. }
+  iApply (intuitionistically_if_mono_iprop with "[] HmΓτ").
+  iIntros "!# [HΓ Hτ]". 
+  iExists w. by iFrame.
 Qed.
