theories/logic/sem_types.v
@@ -82,18 +82,18 @@ Definition sem_ty_uarr `{heapGS Σ}
 
 (* Polymorphic type. *)
 Definition sem_ty_forall `{heapGS Σ} 
-    (C : sem_ty Σ → sem_ty Σ) : sem_ty Σ := 
-    (λ v, ∀ τ, □ EWPW (v <_>)%E {{ v, C τ v }})%I.
+    (m : mode) (C : sem_ty Σ → sem_ty Σ)  : sem_ty Σ := 
+    (λ v, ∀ τ, □? m (EWPW (v <_>)%E {{ v, C τ v }}))%I.
 
 (* Polymorphic effect type. *)
 Definition sem_ty_row_forall `{heapGS Σ} 
-  (A : sem_row Σ → sem_ty Σ) : sem_ty Σ := 
-    (λ v, ∀ θ, □ EWPW (v <_>)%E {{ v, A θ v }})%I.
+  (m : mode) (A : sem_row Σ → sem_ty Σ) : sem_ty Σ := 
+    (λ v, ∀ θ, □? m (EWPW (v <_>)%E {{ v, A θ v }}))%I.
 
 (* Polymorphic type. *)
 Definition sem_ty_mode_forall `{heapGS Σ} 
-    (C : mode → sem_ty Σ) : sem_ty Σ := 
-    (λ v, ∀ ν, □ EWPW (v <_>)%E {{ v, C ν v }})%I.
+  (m : mode) (C : mode → sem_ty Σ) : sem_ty Σ := 
+    (λ v, ∀ ν, □? m (EWPW (v <_>)%E {{ v, C ν v }}))%I.
 
 (* Existential type. *)
 Definition sem_ty_exists `{irisGS eff_lang Σ} 
@@ -143,13 +143,22 @@ Notation "'Ref' τ" := (sem_ty_ref τ%T)
 Notation "'Refᶜ' τ" := (sem_ty_ref_cpy τ%T) 
   (at level 50) : sem_ty_scope.
 
-Notation "'∀T:' α , C " := (sem_ty_forall (λ α, C%T)) 
+Notation "'∀T:' α , C " := (sem_ty_forall MS (λ α, C%T)) 
   (at level 180) : sem_ty_scope.
 
-Notation "'∀R:' θ , C " := (sem_ty_row_forall (λ θ, C%T)) 
+Notation "'∀R:' θ , C " := (sem_ty_row_forall MS (λ θ, C%T)) 
   (at level 180) : sem_ty_scope.
 
-Notation "'∀M:' ν , C " := (sem_ty_mode_forall (λ ν, C%T)) 
+Notation "'∀M:' ν , C " := (sem_ty_mode_forall MS (λ ν, C%T)) 
+  (at level 180) : sem_ty_scope.
+
+Notation "'∀T:[' m ']' α , C " := (sem_ty_forall m (λ α, C%T)) 
+  (at level 180) : sem_ty_scope.
+
+Notation "'∀R:[' m ']' θ , C " := (sem_ty_row_forall m (λ θ, C%T)) 
+  (at level 180) : sem_ty_scope.
+
+Notation "'∀M:[' m ']' ν , C " := (sem_ty_mode_forall m (λ ν, C%T)) 
   (at level 180) : sem_ty_scope.
 
 Notation "'∃:' α , C " := (sem_ty_exists (λ α, C%T)) 
@@ -176,26 +185,6 @@ Notation "τ '-{' ρ '}->' κ" := (sem_ty_uarr ρ%R τ%T κ%T)
   (at level 100, ρ, κ at level 200) : sem_ty_scope.
 Notation "τ → κ" := (sem_ty_uarr ⟨⟩%R τ%T κ%T)
   (at level 99, κ at level 200) : sem_ty_scope.
-
-(* Subsumption relation on rows wrt to types *)
-
-Lemma row_type_sub_copy {Σ} (ρ : sem_row Σ) (τ : sem_ty Σ) : copy_ty τ -∗ ρ ≼ₜ τ.
-Proof.
-  iIntros "#Hτcpy %w %v %Φ !# Hρ Hτ.".
-  iDestruct ("Hτcpy" with "Hτ.") as "#Hτ".
-  iApply (pmono_prot_prop _ (sem_row_car ρ) with "[] Hρ").
-  iIntros "!# % H". iFrame "#". iApply "H".
-Qed.
-
-Lemma row_type_sub_bang {Σ} (ρ : sem_row Σ) (τ : sem_ty Σ) : ⊢ ρ ≼ₜ ('! τ).
-Proof.
-  iIntros (w v Φ) "!# Hρ #Hτ".
-  iApply (pmono_prot_prop _ (sem_row_car ρ) with "[] Hρ").
-  iIntros "!# % $ //".
-Qed.
-
-Lemma row_type_sub_mfbang_mbang {Σ} (m : mode) (ρ : sem_row Σ) (τ : sem_ty Σ) : ⊢ ¡_[ m ] ρ ≼ₜ ('!_[ m ] τ).
-Proof. destruct m; [iApply row_type_sub_fbang|iApply row_type_sub_bang]. Qed.
 
 (* Derived Types *)
 
@@ -252,20 +241,20 @@ Section types_properties.
   Global Instance sem_ty_ref_cpy_ne : NonExpansive (@sem_ty_ref_cpy Σ _).
   Proof. solve_non_expansive. Qed.
 
-  Global Instance sem_ty_forall_ne n :
-    Proper (pointwise_relation _ (dist n) ==> dist n) sem_ty_forall.
+  Global Instance sem_ty_forall_ne m n :
+    Proper (pointwise_relation _ (dist n) ==> dist n) (sem_ty_forall m).
   Proof. intros ????. unfold sem_ty_forall. 
          do 3 f_equiv. f_equiv. by apply non_dep_fun_dist.
   Qed.
 
-  Global Instance sem_ty_forall_row_ne n :
-    Proper (pointwise_relation _ (dist n) ==> dist n) sem_ty_row_forall.
+  Global Instance sem_ty_forall_row_ne m n :
+    Proper (pointwise_relation _ (dist n) ==> dist n) (sem_ty_row_forall m).
   Proof. intros ????. unfold sem_ty_row_forall. 
          do 3 f_equiv. f_equiv. by apply non_dep_fun_dist.
   Qed.
 
-  Global Instance sem_ty_forall_mode_ne n :
-    Proper (pointwise_relation _ (dist n) ==> dist n) sem_ty_mode_forall.
+  Global Instance sem_ty_forall_mode_ne m n :
+    Proper (pointwise_relation _ (dist n) ==> dist n) (sem_ty_mode_forall m).
   Proof. intros ????. unfold sem_ty_mode_forall. 
          do 3 f_equiv. f_equiv. by apply non_dep_fun_dist.
   Qed.
@@ -323,22 +312,22 @@ Section types_properties.
   Global Instance sem_ty_ref_cpy_proper : Proper ((≡) ==> (≡)) (@sem_ty_ref_cpy Σ _).
   Proof. intros ????. unfold sem_ty_ref_cpy; by repeat f_equiv. Qed.
 
-  Global Instance sem_ty_forall_proper :
-    Proper (pointwise_relation _ (≡) ==> (≡)) sem_ty_forall.
+  Global Instance sem_ty_forall_proper m :
+    Proper (pointwise_relation _ (≡) ==> (≡)) (sem_ty_forall m).
   Proof. 
     intros ????. unfold sem_ty_forall; repeat f_equiv. 
     by apply non_dep_fun_equiv. 
   Qed.
 
-  Global Instance sem_ty_row_forall_proper :
-    Proper (pointwise_relation _ (≡) ==> (≡)) sem_ty_row_forall.
+  Global Instance sem_ty_row_forall_proper m :
+    Proper (pointwise_relation _ (≡) ==> (≡)) (sem_ty_row_forall m).
   Proof. 
     intros ????. unfold sem_ty_row_forall; repeat f_equiv. 
     by apply non_dep_fun_equiv. 
   Qed.
 
-  Global Instance sem_ty_mode_forall_proper :
-    Proper (pointwise_relation _ (≡) ==> (≡)) sem_ty_mode_forall.
+  Global Instance sem_ty_mode_forall_proper m :
+    Proper (pointwise_relation _ (≡) ==> (≡)) (sem_ty_mode_forall m).
   Proof. 
     intros ????. unfold sem_ty_mode_forall; repeat f_equiv. 
     by apply non_dep_fun_equiv. 
@@ -358,7 +347,178 @@ Section types_properties.
     apply sem_ty_rec_ne=> A. by apply equiv_dist.
   Qed.
 
+  Global Instance sem_ty_uarr_persistent `{heapGS Σ} (τ κ : sem_ty Σ) (ρ : sem_row Σ) v :
+    Persistent ((sem_ty_uarr ρ τ κ) v).
+  Proof.
+    rewrite /sem_ty_uarr /sem_ty_arr. simpl. apply _.
+  Qed.
+
+  Global Instance sem_ty_forall_type_persistent `{heapGS Σ} (C : sem_ty Σ → sem_ty Σ) v :
+    Persistent ((sem_ty_forall MS C) v).
+  Proof.
+    unfold sem_ty_forall. simpl. apply _.
+  Qed.
+
+  Global Instance sem_ty_row_forall_persistent `{heapGS Σ} (C : sem_row Σ → sem_ty Σ) v :
+    Persistent ((sem_ty_row_forall MS C) v).
+  Proof.
+    unfold sem_ty_row_forall. simpl. apply _.
+  Qed.
+
+  Global Instance sem_ty_mode_forall_persistent `{heapGS Σ} (C : mode → sem_ty Σ) v :
+    Persistent ((sem_ty_mode_forall MS C) v).
+  Proof.
+    unfold sem_ty_mode_forall. simpl. apply _.
+  Qed.
+
 End types_properties.
+
+Section copyable_types.
+  
+  Context `{heapGS Σ}.
+
+  Implicit Types τ κ : sem_ty Σ.
+
+  (* Copyable types *)
+  
+  Open Scope sem_ty_scope.
+
+  Lemma copy_ty_void : ⊢ @copy_ty Σ Void.
+  Proof. iIntros "!# %v $!". Qed.
+
+  Lemma copy_ty_unit : ⊢ @copy_ty Σ ().
+  Proof. iIntros "!# %v $!". Qed.
+  
+  Lemma copy_ty_bool : ⊢ @copy_ty Σ 𝔹.
+  Proof. iIntros "!# %v #$". Qed.
+  
+  Lemma copy_ty_nat : ⊢ @copy_ty Σ ℤ.
+  Proof. iIntros "!# %v #$". Qed.
+  
+  Lemma copy_ty_top : ⊢ @copy_ty Σ ⊤.
+  Proof. iIntros "!# %v #$". Qed.
+
+  Lemma copy_ty_bang τ : ⊢ copy_ty ('! τ).
+  Proof. iIntros "!# %v #$". Qed.
+
+  Lemma copy_ty_uarr τ σ κ : ⊢ copy_ty (τ -{ σ }-> κ).
+  Proof. 
+    rewrite /sem_ty_uarr /sem_ty_arr /=.
+    iIntros "/= !# %v #$". 
+  Qed.
+  
+  Lemma copy_ty_prod τ κ : copy_ty τ -∗ copy_ty κ -∗ copy_ty (τ × κ).
+  Proof. 
+    iIntros "#Hcpyτ #Hcpyκ !# %v (% & % & -> & Hτ & Hκ)". 
+    iDestruct ("Hcpyτ" with "Hτ") as "#Hτ'".
+    iDestruct ("Hcpyκ" with "Hκ") as "#Hκ'". 
+    iIntros "!#". iExists v₁, v₂. by iFrame "#".
+  Qed.
+
+  Lemma copy_ty_sum τ κ : copy_ty τ -∗ copy_ty κ -∗ copy_ty (τ + κ).
+  Proof.
+    iIntros "#Hcpyτ #Hcpyκ !# %v (% & [(-> & Hτ)|(-> & Hκ)])". 
+    - iDestruct ("Hcpyτ" with "Hτ") as "#Hτ'". iIntros "!#". 
+      iExists v'. iLeft. by iFrame "#".
+    - iDestruct ("Hcpyκ" with "Hκ") as "#Hκ'". iIntros "!#". 
+      iExists v'. iRight. by iFrame "#".
+  Qed.
+
+  Lemma copy_ty_forallT C : ⊢ copy_ty (∀T: α, C α).
+  Proof. iIntros "!# % #$". Qed.
+
+  Lemma copy_ty_forallR C : ⊢ copy_ty (∀R: θ, C θ).
+  Proof. iIntros "!# % #$". Qed.
+
+  Lemma copy_ty_forallM C : ⊢ copy_ty (∀M: ν, C ν).
+  Proof. iIntros "!# % #$". Qed.
+
+  Lemma copy_ty_ref τ : ⊢ copy_ty (Refᶜ τ).
+  Proof. iIntros "!# % #$". Qed.
+
+  Lemma copy_ty_exists A : (∀ α, copy_ty (A α)) -∗ copy_ty (∃: α, A α).
+  Proof. 
+    iIntros "#H !# % [%α Hτ']". 
+    iDestruct ("H" with "Hτ'") as "#Hτ".
+    iIntros "!#". by iExists α.
+  Qed.
+
+  Lemma copy_ty_rec A `{NonExpansive A}: 
+    □ (∀ α, (copy_ty α) -∗ copy_ty (A α)) -∗ 
+    @copy_ty Σ (μT: α, A α).
+  Proof. 
+    iIntros "#H !# %". iLöb as "IH" forall (v). 
+    rewrite {1 2} sem_ty_rec_unfold.
+    iIntros "Hτ". iApply bi.later_intuitionistically.
+    iNext. iApply ("H" with "[] Hτ"). 
+    rewrite /copy_ty /tc_opaque. iApply "IH".
+  Qed.
+
+  Lemma copy_ty_option τ : copy_ty τ -∗ copy_ty (Option τ).
+  Proof. 
+    iIntros "#H". 
+    iApply copy_ty_sum; [iApply copy_ty_unit|done]. 
+  Qed.
+
+  Lemma copy_ty_list τ : copy_ty τ -∗ copy_ty (List τ).
+  Proof.
+    iIntros "#Hτ". iApply copy_ty_rec.
+    iIntros "!# % #Hα". 
+    iApply copy_ty_sum; [iApply copy_ty_unit|].
+    by iApply copy_ty_prod.
+  Qed.
+
+  Lemma copy_env_nil : ⊢ @copy_env Σ [].
+  Proof. iIntros "!# % #$". Qed.
+  
+  Lemma copy_env_cons Γ x τ : 
+    copy_env Γ -∗
+    copy_ty τ -∗
+    copy_env ((x, τ) :: Γ).
+  Proof. 
+    iIntros "#HΓcpy #Hτcpy !# % (% & %Hrw & Hτ & HΓ)".
+    iDestruct ("Hτcpy" with "Hτ") as "#Hτ'".
+    iDestruct ("HΓcpy" with "HΓ") as "#HΓ'".
+    iIntros "!#". iExists v. by iFrame "#".
+  Qed.
+
+End copyable_types.
+
+Section type_sub.
+
+(* Subsumption relation on modes and rows wrt to types *)
+
+Lemma row_type_sub_copy {Σ} (ρ : sem_row Σ) (τ : sem_ty Σ) : copy_ty τ -∗ ρ ≼ₜ τ.
+Proof.
+  iIntros "#Hτcpy %w %v %Φ !# Hρ Hτ.".
+  iDestruct ("Hτcpy" with "Hτ.") as "#Hτ".
+  iApply (pmono_prot_prop _ (sem_row_car ρ) with "[] Hρ").
+  iIntros "!# % H". iFrame "#". iApply "H".
+Qed.
+
+Lemma row_type_sub_bang {Σ} (ρ : sem_row Σ) (τ : sem_ty Σ) : ⊢ ρ ≼ₜ ('! τ).
+Proof.
+  iIntros (w v Φ) "!# Hρ #Hτ".
+  iApply (pmono_prot_prop _ (sem_row_car ρ) with "[] Hρ").
+  iIntros "!# % $ //".
+Qed.
+
+Lemma row_type_sub_mfbang_mbang {Σ} (m : mode) (ρ : sem_row Σ) (τ : sem_ty Σ) : ⊢ ¡_[ m ] ρ ≼ₜ ('!_[ m ] τ).
+Proof. destruct m; [iApply row_type_sub_fbang|iApply row_type_sub_bang]. Qed.
+
+Lemma mode_type_sub_mbang {Σ} m (τ : sem_ty Σ) : ⊢ m ₘ≼ₜ '!_[m] τ.
+Proof. 
+  rewrite /mode_type_sub /=. iIntros "!# % Hτ". 
+  destruct m; simpl; first done. iApply "Hτ".
+Qed.
+
+Lemma mode_type_sub_mbang_meet {Σ} (m m' : mode) (τ : sem_ty Σ) : ⊢ m ⊓ₘ m' ₘ≼ₜ ('!_[ m ] τ).
+Proof. 
+  destruct m; first rewrite mode_glb_os; first iApply mode_type_sub_os.
+  iApply mode_type_sub_ms. iApply copy_ty_bang.
+Qed.
+
+End type_sub.
 
 Section sub_typing.
 
@@ -380,11 +540,13 @@ Section sub_typing.
     ⊢ Void ≤T τ.
   Proof. iIntros "% !# []". Qed.
 
-  Lemma ty_le_bang_intro (τ : sem_ty Σ) :
+  Lemma ty_le_mbang_intro m (τ : sem_ty Σ) :
     copy_ty τ -∗
-    τ ≤T '! τ.
+    τ ≤T '!_[m] τ.
   Proof. 
-    iIntros "#Hcpy !# %v Hτ". 
+    iIntros "#Hcpy".
+    destruct m; simpl; first iApply ty_le_refl.
+    iIntros "!# %v Hτ". 
     iDestruct ("Hcpy" with "Hτ") as "#Hτ'".
     iIntros "!# {$#Hτ'}". 
   Qed.
@@ -402,8 +564,38 @@ Section sub_typing.
     by iApply "Hττ'".
   Qed.
 
+  Lemma ty_le_mbang_idemp_intro m (τ : sem_ty Σ) :
+    ⊢ '!_[m] τ ≤T '!_[m] ('!_[m] τ).
+  Proof. 
+    destruct m; simpl; first iApply ty_le_refl.
+    iApply (ty_le_mbang_intro MS). iApply copy_ty_bang.
+  Qed.
+
+  Lemma ty_le_mbang_comm m m' (τ : sem_ty Σ) :
+    ⊢ '!_[m] ('!_[m'] τ) ≤T '!_[m'] ('!_[m] τ). 
+  Proof. 
+    destruct m, m'; iApply ty_le_refl.
+  Qed.
+
+  Lemma ty_le_mbang_mode_le m m' (τ : sem_ty Σ) :
+    ⊢ m' ≤M m -∗ ('!_[m] τ) ≤T ('!_[m'] τ). 
+  Proof. 
+    iIntros "H". destruct m.
+    - iDestruct (mode_le_OS_inv with "H") as "->".
+      iApply ty_le_refl.
+    - destruct m'; [iApply (ty_le_mbang_elim MS)|iApply ty_le_refl].
+Qed.
+
+  Lemma ty_le_mbang_arr_intro (τ κ : sem_ty Σ) (ρ : sem_row Σ) (m : mode) :
+    ⊢ (τ -{ ρ }-[ m ]-> κ) ≤T '!_[m] (τ -{ ρ }-[ m ]-> κ).
+  Proof.
+    iIntros. destruct m; simpl; first iApply ty_le_refl.
+    iApply (ty_le_mbang_intro MS).
+    iApply copy_ty_uarr.
+  Qed.
+
   Lemma ty_le_arr (τ₁ κ₁ τ₂ κ₂ : sem_ty Σ) (ρ ρ' : sem_row Σ) (m m' : mode) :
-    m ≤M m' -∗
+    m' ≤M m -∗
     ρ ≤R ρ' -∗
     τ₂ ≤T τ₁ -∗
     κ₁ ≤T κ₂ -∗
@@ -412,15 +604,16 @@ Section sub_typing.
     iIntros "#Hm #Hρ  #Hτ₂₁ #Hκ₁₂ !# %v Hτκ₁". 
     destruct m.
     - iDestruct "Hm" as "[<-|%H]"; last inv H.  
-      rewrite /sem_ty_arr /=. iIntros "%w Hτ₂".
+      rewrite /sem_ty_arr /=. 
+      iApply (intuitionistically_if_mono_iprop with "[] Hτκ₁").
+      iIntros "!# Hτκ₁ % Hτ₂".
       iApply (ewpw_sub with "Hρ").
       iApply (ewpw_mono with "[Hτκ₁ Hτ₂]").
       { iApply ("Hτκ₁" with "[Hτ₂]"); by iApply "Hτ₂₁". }
       iIntros "!# % Hκ !>". by iApply "Hκ₁₂".
     - rewrite /sem_ty_arr /=.  
       iApply bi.intuitionistically_intuitionistically_if.
-      iDestruct "Hτκ₁" as "#Hτκ₁".
-      iIntros "!# %w Hτ₂".
+      iDestruct "Hτκ₁" as "#Hτκ₁". iIntros "!# %w Hτ₂".
       iApply (ewpw_sub with "Hρ").
       iApply (ewpw_mono with "[Hτκ₁ Hτ₂]").
       { iApply ("Hτκ₁" with "[Hτ₂]"); by iApply "Hτ₂₁". }
@@ -474,6 +667,17 @@ Section sub_typing.
     by iApply "Hκ₁₂".
   Qed.
   
+  Lemma ty_le_mbang_prod_intro m (τ κ : sem_ty Σ) :
+    τ ≤T '!_[m] τ -∗
+    κ ≤T '!_[m] κ -∗
+    (τ × κ) ≤T '!_[m] (τ × κ).
+  Proof.
+    iIntros "#Hτ #Hκ". 
+    destruct m; simpl; first iApply ty_le_refl.
+    iApply (ty_le_mbang_intro MS).
+    iApply (copy_ty_prod with "Hτ Hκ").
+  Qed.
+
   Lemma ty_le_sum (τ₁ τ₂ κ₁ κ₂ : sem_ty Σ) :
     τ₁ ≤T τ₂ -∗
     κ₁ ≤T κ₂ -∗
@@ -484,38 +688,77 @@ Section sub_typing.
     - iRight. iSplit; first done. by iApply "Hκ₁₂". 
   Qed.
 
+  Lemma ty_le_mbang_sum_intro m (τ κ : sem_ty Σ) :
+    τ ≤T '!_[m] τ -∗
+    κ ≤T '!_[m] κ -∗
+    (τ + κ) ≤T '!_[m] (τ + κ).
+  Proof.
+    iIntros "#Hτ #Hκ". 
+    destruct m; simpl; first iApply ty_le_refl.
+    iApply (ty_le_mbang_intro MS).
+    iApply (copy_ty_sum with "Hτ Hκ").
+  Qed.
+
   Lemma ty_le_option (τ₁ τ₂ : sem_ty Σ) :
     τ₁ ≤T τ₂ -∗
     (Option τ₁) ≤T (Option τ₂).
   Proof. iIntros "#?". iApply ty_le_sum; last done. iIntros "!# % $". Qed.
 
-  Lemma ty_le_forall (τ₁ τ₂ : sem_ty Σ → sem_ty Σ) :
+  Lemma ty_le_forall m (τ₁ τ₂ : sem_ty Σ → sem_ty Σ) :
     (∀ α, τ₁ α ≤T τ₂ α) -∗
-    (∀T: α, τ₁ α)%T ≤T (∀T: α, τ₂ α).
+    (∀T:[m] α, τ₁ α)%T ≤T (∀T:[m] α, τ₂ α).
   Proof.
-    iIntros "#Hτ₁₂ !# %v #Hτ₁ %τ !#".
-    iApply (ewpw_mono with "[Hτ₁]"); [iApply "Hτ₁"|].
-    iIntros "!# % Hτ !>". by iApply "Hτ₁₂".
+    iIntros "#Hτ₁₂ !# %v". destruct m; simpl. 
+    - iIntros "Hτ₁ %τ /=". iApply (ewpw_mono with "[Hτ₁]"); [iApply "Hτ₁"|].
+      iIntros "!# % Hτ !>". by iApply "Hτ₁₂".
+    - iIntros "#Hτ₁ %τ /= !#". rewrite /sem_ty_forall /=.
+      iApply (ewpw_mono with "[Hτ₁]"); [iApply "Hτ₁"|].
+      iIntros "!# % Hτ !>". by iApply "Hτ₁₂".
   Qed.
 
-  Lemma ty_le_row_forall (τ₁ τ₂ : sem_row Σ → sem_ty Σ) :
+  Lemma ty_le_mbang_forall_intro m (τ : sem_ty Σ → sem_ty Σ) :
+    ⊢ (∀T:[m] α, τ α)%T ≤T '!_[m] (∀T:[m] α, τ α).
+  Proof.
+    destruct m; simpl; first iApply ty_le_refl.
+    iApply (ty_le_mbang_intro MS); iApply copy_ty_forallT.
+  Qed.
+
+  Lemma ty_le_row_forall m (τ₁ τ₂ : sem_row Σ → sem_ty Σ) :
     (∀ θ, τ₁ θ ≤T τ₂ θ) -∗
-    (∀R: θ, τ₁ θ) ≤T (∀R: θ, τ₂ θ).
+    (∀R:[m] θ, τ₁ θ) ≤T (∀R:[m] θ, τ₂ θ).
   Proof.
-    iIntros "#Hτ₁₂ !# %v #Hτ₁ %σ !#".
-    iApply (ewpw_mono with "[Hτ₁]"); [iApply "Hτ₁"|].
-    iIntros "!# % Hτ₁σ !>".
-    iApply ("Hτ₁₂" $! σ with "Hτ₁σ").
+    iIntros "#Hτ₁₂ !# %v". destruct m; simpl. 
+    - iIntros "Hτ₁ %τ /=". iApply (ewpw_mono with "[Hτ₁]"); [iApply "Hτ₁"|].
+      iIntros "!# % Hτ !>". by iApply "Hτ₁₂".
+    - iIntros "#Hτ₁ %τ /= !#". rewrite /sem_ty_row_forall /=. 
+      iApply (ewpw_mono with "[Hτ₁]"); [iApply "Hτ₁"|].
+      iIntros "!# % Hτ !>". by iApply "Hτ₁₂".
   Qed.
 
-  Lemma ty_le_mode_forall (τ₁ τ₂ : mode → sem_ty Σ) :
-    (∀ ν, τ₁ ν ≤T τ₂ ν) -∗
-    (∀M: ν, τ₁ ν) ≤T (∀M: ν, τ₂ ν).
+  Lemma ty_le_mbang_row_forall_intro m (τ : sem_row Σ → sem_ty Σ) :
+    ⊢ (∀R:[m] θ, τ θ)%T ≤T '!_[m] (∀R:[m] θ, τ θ).
   Proof.
-    iIntros "#Hτ₁₂ !# %v #Hτ₁ %σ !#".
-    iApply (ewpw_mono with "[Hτ₁]"); [iApply "Hτ₁"|].
-    iIntros "!# % Hτ₁σ !>".
-    iApply ("Hτ₁₂" $! σ with "Hτ₁σ").
+    destruct m; simpl; first iApply ty_le_refl.
+    iApply (ty_le_mbang_intro MS); iApply copy_ty_forallR.
+  Qed.
+
+  Lemma ty_le_mode_forall m (τ₁ τ₂ : mode → sem_ty Σ) :
+    (∀ ν, τ₁ ν ≤T τ₂ ν) -∗
+    (∀M:[m] ν, τ₁ ν) ≤T (∀M:[m] ν, τ₂ ν).
+  Proof.
+    iIntros "#Hτ₁₂ !# %v". destruct m; simpl. 
+    - iIntros "Hτ₁ %τ /=". iApply (ewpw_mono with "[Hτ₁]"); [iApply "Hτ₁"|].
+      iIntros "!# % Hτ !>". by iApply "Hτ₁₂".
+    - iIntros "#Hτ₁ %τ /= !#". rewrite /sem_ty_mode_forall /=. 
+      iApply (ewpw_mono with "[Hτ₁]"); [iApply "Hτ₁"|].
+      iIntros "!# % Hτ !>". by iApply "Hτ₁₂".
+  Qed.
+
+  Lemma ty_le_mbang_mode_forall_intro m (τ : mode → sem_ty Σ) :
+    ⊢ (∀M:[m] ν, τ ν)%T ≤T '!_[m] (∀M:[m] ν, τ ν).
+  Proof.
+    destruct m; simpl; first iApply ty_le_refl.
+    iApply (ty_le_mbang_intro MS); iApply copy_ty_forallM.
   Qed.
 
   Lemma ty_le_exists (τ₁ τ₂ : sem_ty Σ → sem_ty Σ) :
@@ -536,6 +779,25 @@ Section sub_typing.
     iApply ("Hτ₁₂" with "[] Hτ₁").
     rewrite /ty_le /tc_opaque. iApply "IH".
   Qed.
+  
+  Lemma ty_le_rec_bang m (τ : sem_ty Σ -> sem_ty Σ) `{NonExpansive τ} :
+    □ (∀ α, (α ≤T '!_[m] α) -∗ τ α ≤T '!_[m] (τ α)) -∗
+    (μT: α, τ α) ≤T '!_[m] (μT: α, τ α).
+  Proof. 
+    iIntros "#H". 
+    destruct m; simpl; first iApply ty_le_refl.
+    iIntros "!# %v Hτα".
+    iLöb as "IH" forall (v).
+    rewrite {1} sem_ty_rec_unfold.
+    assert (fixpoint (sem_ty_rec_pre τ) v ≡ sem_ty_rec_pre τ (fixpoint (sem_ty_rec_pre τ)) v).
+    { apply non_dep_fun_equiv. apply fixpoint_unfold. }
+    rewrite {4} /sem_ty_rec /sem_ty_bang H {1} /sem_ty_rec_pre.
+    iApply bi.later_intuitionistically. iNext. iExists (fixpoint (sem_ty_rec_pre τ)).
+    iSpecialize ("H" $! (μT: α, τ α)%T with "[IH]").
+    { iIntros "% !# //". }
+    iDestruct ("H" $! v with "Hτα") as "#Hτα'". iIntros "!#".
+    iSplit; first done. iApply "Hτα'".
+  Qed.
 
   Lemma ty_le_list (τ₁ τ₂ : sem_ty Σ) :
     τ₁ ≤T τ₂ -∗
@@ -550,6 +812,17 @@ Section sub_typing.
     iExists (w₁, w₂)%V. iRight. iSplit; first done.
     iExists w₁, w₂; iSplit; first done.
     iSplitL "Hτ₁"; [by iApply "Hτ₁₂"|by iApply "IH"].
+  Qed.
+
+  Lemma ty_le_list_bang m (τ : sem_ty Σ) :
+    ⊢ List ('!_[m] τ) ≤T '!_[m] (List ('!_[m] τ)).
+  Proof.
+    rewrite /sem_ty_list /ListF. iIntros.
+    iApply ty_le_rec_bang. iIntros "!# %α #Hle".
+    iApply ty_le_mbang_sum_intro.
+    { iApply ty_le_mbang_intro. iApply copy_ty_unit. }
+    iApply (ty_le_mbang_prod_intro with "[] Hle").
+    iApply ty_le_mbang_idemp_intro.
   Qed.
   
 End sub_typing.
