theories/case_studies/cooperative_concurrency_gen.v
@@ -19,7 +19,7 @@ From affect.logic Require Import sem_env.
 From affect.logic Require Import sem_sig.
 From affect.logic Require Import sem_row.
 From affect.logic Require Import sem_types.
-From affect.logic Require Import copyable.
+From affect.logic Require Import mode.
 From affect.logic Require Import sem_judgement.
 From affect.logic Require Import sem_operators.
 From affect.logic Require Import compatibility.
@@ -269,7 +269,7 @@ Section typing.
       + iApply sem_typed_sub_nil.
         rewrite - {1} (app_nil_r []).
         iApply sem_typed_afun; solve_sidecond. simpl.
-        iApply sem_typed_sub_ty; [iApply ty_le_bang_intro; solve_copy|].
+        iApply sem_typed_sub_ty; [iApply (ty_le_mbang_intro MS); solve_copy|].
         iApply sem_typed_unit'.
   Qed.
 
@@ -350,7 +350,9 @@ Section typing.
     iIntros. rewrite /resume_task_ty.
     iApply sem_typed_closure; solve_sidecond. simpl.
     set add := ("add", add_ty θ')%T. rewrite -(app_nil_r [add]).
-    iApply sem_typed_TLam; solve_sidecond. iIntros (α).
+    iApply sem_typed_TLam; solve_sidecond. 
+    { iApply mode_env_sub_cons; first iApply mode_env_sub_ms; solve_copy. }
+    iIntros (α).
     rewrite -(app_nil_r [add]).
     iApply sem_typed_ufun; solve_sidecond. simpl.
     rewrite -(app_nil_r [("v", '! α); add]).
@@ -526,7 +528,7 @@ Section typing.
             [iApply (row_le_mfbang_intro OS)|iApply ty_le_refl|iApply ty_le_refl|].
            iApply sem_typed_sub_ty; first iApply ty_le_uarr; 
             [iApply row_le_refl|iApply ty_le_refl|iApply ty_le_aarr|];
-            [iApply row_le_fbang_elim|iApply ty_le_refl|iApply ty_le_refl|].
+            [iApply (row_le_mfbang_elim OS)|iApply ty_le_refl|iApply ty_le_refl|].
             set C := (λ (θ : sem_row Σ), (('! β -{ θ' }-∘ ()) -{ ¡ θ }-> ()) → List ('! β -{θ'}-∘ ()) -{ ¡ θ }-∘ ())%T.
            rewrite -/(C ⊥).
            iApply sem_typed_RApp; first solve_copy. 
@@ -565,7 +567,7 @@ Section typing.
     - iApply sem_typed_sub_ty; first iApply ty_le_u2aarr.
       iApply sem_typed_sub_ty.
       { iApply ty_le_uarr; [iApply row_le_refl| |iApply (ty_le_mbang_elim MS)].
-        iApply ty_le_aarr; [iApply row_le_refl|iApply ty_le_refl|iApply ty_le_bang_intro; solve_copy]. }
+        iApply ty_le_aarr; [iApply row_le_refl|iApply ty_le_refl|iApply (ty_le_mbang_intro MS); solve_copy]. }
       set R := (λ α θ', (() -{ coop θ' }-∘ '! α) -{ θ' }-> '! α)%T.
       rewrite /coopstate -/(R () st).
       iApply (sem_typed_RApp (R ())).
@@ -597,7 +599,7 @@ Section typing.
           rewrite -/(coop st) {1} /coop_pre {7} /st.
           iApply sem_typed_sub_row; first iApply row_le_swap_third; try done.
           iApply sem_typed_sub_row; first iApply row_le_swap_second; try done.
-          iApply sem_typed_sub_ty; first iApply ty_le_bang_intro; first solve_copy.
+          iApply sem_typed_sub_ty; first iApply (ty_le_mbang_intro MS); first solve_copy.
           iApply (sem_typed_perform_ms (TT:=[tele _]) [tele_arg ()] with "[] []"); solve_sidecond.
           iApply sem_typed_sub_row; first iApply row_le_swap_fourth; try done.
           do 2 (iApply sem_typed_sub_row; first iApply row_le_swap_third; try done).
