theories/case_studies/tossCoin.v
@@ -19,7 +19,6 @@ From affect.logic Require Import sem_sig.
 From affect.logic Require Import sem_row.
 From affect.logic Require Import sem_types.
 From affect.logic Require Import sem_judgement.
-From affect.logic Require Import copyable.
 From affect.logic Require Import sem_operators.
 From affect.logic Require Import compatibility.
 From affect.logic Require Import tactics.
